we can now vm_compute the bedrock2-compiled IncrementWait
example on the deterministic riscv-coq machine with a
Cava increment circuit attached

investigations/bedrock2/RiscvMachineWithCavaDevice/DetIncrMachine.v
@@ -8,7 +8,7 @@ Section WithCava.
 
   Definition ite{T: SignalType}(cond: signal Bit)(thn els: signal T):
     cava (signal T) :=
-    branches <- packV (Vector.of_list [thn; els]);;
+    branches <- packV (Vector.of_list [els; thn]);;
     ctrl <- packV (Vector.of_list [cond]);;
     indexAt branches ctrl.
 
@@ -19,7 +19,9 @@ Section WithCava.
       done <- Vec.hd state;;
       value <- Vec.tl state;;
       done' <- ret (constant true);;
-      value_plus_one <- incrN value;;
+      value_r <- Vec.rev value;;
+      value_plus_one_r <- incrN value_r;;
+      value_plus_one <- Vec.rev value_plus_one_r;;
       value' <- ite done value value_plus_one;;
       state' <- Vec.cons done' value';;
       ret (tt, state').
@@ -30,32 +32,41 @@ End WithCava.
 
 Definition device_state := Vector.t bool 32.
 
+(*
 Eval simpl in circuit_state incr.
+*)
 
 Definition incr_device_step(state: device_state): device_state :=
   snd (snd (fst (step incr (tt, (tt, state)) tt))).
+
+(*
+Compute incr_device_step (Vector.const false 1 ++ Vector.const false 28 ++ Vector.const true 3)%vector.
+*)
 
 Require Import Coq.ZArith.ZArith. Open Scope Z_scope.
 Require Import riscv.Utility.Utility.
 Require Import coqutil.Map.Interface.
 Require Import coqutil.Map.Properties.
-Require Import Bedrock2Experiments.RiscvMachineWithCavaDevice.ExtraMMIORiscvMachine.
 Require Import Bedrock2Experiments.RiscvMachineWithCavaDevice.InternalMMIOMachine.
 
 Section WithParameters.
   Context {word: Interface.word 32} {word_ok: word.ok word}
           {Mem: map.map word byte} {Registers: map.map Z word}.
 
-  Definition INCR_DEVICE_ADDR: word := word.of_Z 0x10000.
+  Definition INCR_DEVICE_ADDR: word := word.of_Z (16 * 2^10).
+
+  (* we want the msb to be the head, and we use Cava's reverse rather than Coq's reverse
+     because Coq's contains opaque proof terms *)
 
   Definition bv_to_word(v: Vector.t bool 32): word :=
-    word.of_Z (Z.of_N (Bv2N v)).
+    word.of_Z (Z.of_N (Bv2N (Cava.Util.Vector.reverse v))).
 
   Definition word_to_bv(w: word): Vector.t bool 32 :=
-    N2Bv_sized 32 (Z.to_N (word.unsigned w)).
+    Cava.Util.Vector.reverse (N2Bv_sized 32 (Z.to_N (word.unsigned w))).
 
   Global Instance counter_device: device := {|
     device.state := device_state;
+    device.reset_state := word_to_bv (word.of_Z 0);
     device.run1 := incr_device_step;
     device.addr_range_start := INCR_DEVICE_ADDR;
     device.addr_range_pastend := word.add INCR_DEVICE_ADDR (word.of_Z 4);
