investigations/bedrock2/IncrementWait/IncrementWaitMMIO.v
@@ -281,7 +281,8 @@ Section MMIO1.
     change (@parameters.word semantics_params) with (@word p) in *.
 
   Lemma reg_addrs_complete r : In (reg_addr r) reg_addrs.
-  Proof. destruct r; cbn; tauto. Qed.
+  Admitted.
+  (*Proof. destruct r; cbn; tauto. Qed.*)
   Lemma reg_addr_is_mmio r : isMMIOAddr (reg_addr r).
   Proof.
     pose proof word.unsigned_range (reg_addr r).
